tacenta-proofs/translation/Translation/TacentaSessionUnit.lean
@@ -389,16 +389,6 @@ axiom alloc.vec.Vec.pop
   {T : Type} (A : Type) :
   alloc.vec.Vec T → Result ((Option T) × (alloc.vec.Vec T))
 
-/-- [alloc::vec::{alloc::vec::Vec<T>}::append]:
-    Source: '/rustc/library/alloc/src/vec/mod.rs', lines 2927:4-2927:46
-    Name pattern: [alloc::vec::{alloc::vec::Vec<@T>}::append]
-    Visibility: public -/
-@[rust_fun "alloc::vec::{alloc::vec::Vec<@T>}::append"]
-axiom alloc.vec.Vec.append
-  {T : Type} (A : Type) :
-  alloc.vec.Vec T → alloc.vec.Vec T → Result ((alloc.vec.Vec T) ×
-    (alloc.vec.Vec T))
-
 /-- [alloc::vec::{alloc::vec::Vec<T>}::is_empty]:
     Source: '/rustc/library/alloc/src/vec/mod.rs', lines 3085:4-3085:40
     Name pattern: [alloc::vec::{alloc::vec::Vec<@T>}::is_empty]
@@ -6587,7 +6577,7 @@ def tacenta_spqr.State.invariant
   else ok false
 
 /-- [tacenta_session_unit::tacenta_spqr::{tacenta_session_unit::tacenta_spqr::State}::remove_skipped_at]: loop body 0:
-    Source: 'session-unit/src/../../spqr/src/lib.rs', lines 672:8-675:9 -/
+    Source: 'session-unit/src/../../spqr/src/lib.rs', lines 692:8-695:9 -/
 @[rust_loop_body]
 def tacenta_spqr.State.remove_skipped_at_loop.body
   (skipped : alloc.vec.Vec tacenta_spqr.Skipped) (i : Std.Usize) :
@@ -6605,7 +6595,7 @@ def tacenta_spqr.State.remove_skipped_at_loop.body
   else ok (done (skipped, i))
 
 /-- [tacenta_session_unit::tacenta_spqr::{tacenta_session_unit::tacenta_spqr::State}::remove_skipped_at]: loop 0:
-    Source: 'session-unit/src/../../spqr/src/lib.rs', lines 672:8-675:9 -/
+    Source: 'session-unit/src/../../spqr/src/lib.rs', lines 692:8-695:9 -/
 @[rust_loop]
 def tacenta_spqr.State.remove_skipped_at_loop
   (skipped : alloc.vec.Vec tacenta_spqr.Skipped) (i : Std.Usize) :
@@ -6617,7 +6607,7 @@ def tacenta_spqr.State.remove_skipped_at_loop
     (skipped, i)
 
 /-- [tacenta_session_unit::tacenta_spqr::{tacenta_session_unit::tacenta_spqr::State}::remove_skipped_at]:
-    Source: 'session-unit/src/../../spqr/src/lib.rs', lines 670:4-680:5 -/
+    Source: 'session-unit/src/../../spqr/src/lib.rs', lines 690:4-700:5 -/
 def tacenta_spqr.State.remove_skipped_at
   (skipped : alloc.vec.Vec tacenta_spqr.Skipped) (index : Std.Usize) :
   Result ((Array Std.U8 32#usize) × (alloc.vec.Vec tacenta_spqr.Skipped))
@@ -6681,13 +6671,72 @@ def tacenta_spqr.State.evict_oldest
   := do
   tacenta_spqr.State.evict_oldest_loop self count 0#usize
 
+/-- [tacenta_session_unit::tacenta_spqr::{tacenta_session_unit::tacenta_spqr::State}::prepare_chains_capacity]: loop body 0:
+    Source: 'session-unit/src/../../spqr/src/lib.rs', lines 566:8-569:9 -/
+@[rust_loop_body]
+def tacenta_spqr.State.prepare_chains_capacity_loop.body
+  (v : alloc.vec.Vec (Std.U64 × tacenta_spqr.Chains))
+  (replacement : alloc.vec.Vec (Std.U64 × tacenta_spqr.Chains))
+  (i : Std.Usize) :
+  Result (ControlFlow ((alloc.vec.Vec (Std.U64 × tacenta_spqr.Chains)) ×
+    Std.Usize) (alloc.vec.Vec (Std.U64 × tacenta_spqr.Chains)))
+  := do
+  let i1 := alloc.vec.Vec.len v
+  if i < i1
+  then
+    let p ←
+      alloc.vec.Vec.index (core.slice.index.SliceIndexUsizeSlice (Std.U64 ×
+        tacenta_spqr.Chains)) v i
+    let p1 ← (BuiltinClone (Std.U64 × tacenta_spqr.Chains)).clone p
+    let replacement1 ← alloc.vec.Vec.push replacement p1
+    let i2 ← i + 1#usize
+    ok (cont (replacement1, i2))
+  else ok (done replacement)
+
+/-- [tacenta_session_unit::tacenta_spqr::{tacenta_session_unit::tacenta_spqr::State}::prepare_chains_capacity]: loop 0:
+    Source: 'session-unit/src/../../spqr/src/lib.rs', lines 566:8-569:9 -/
+@[rust_loop]
+def tacenta_spqr.State.prepare_chains_capacity_loop
+  (v : alloc.vec.Vec (Std.U64 × tacenta_spqr.Chains))
+  (replacement : alloc.vec.Vec (Std.U64 × tacenta_spqr.Chains))
+  (i : Std.Usize) :
+  Result (alloc.vec.Vec (Std.U64 × tacenta_spqr.Chains))
+  := do
+  loop
+    (fun (replacement1, i1) =>
+      tacenta_spqr.State.prepare_chains_capacity_loop.body v replacement1 i1)
+    (replacement, i)
+
+/-- [tacenta_session_unit::tacenta_spqr::{tacenta_session_unit::tacenta_spqr::State}::prepare_chains_capacity]:
+    Source: 'session-unit/src/../../spqr/src/lib.rs', lines 559:4-572:5 -/
+def tacenta_spqr.State.prepare_chains_capacity
+  (self : tacenta_spqr.State) (additional : Std.Usize) :
+  Result tacenta_spqr.State
+  := do
+  let i := alloc.vec.Vec.len self.chains
+  let required ← lift (core.num.Usize.saturating_add i additional)
+  let i1 ← alloc.vec.Vec.capacity Global self.chains
+  if required <= i1
+  then ok self
+  else
+    let replacement :=
+      alloc.vec.Vec.with_capacity (Std.U64 × tacenta_spqr.Chains) required
+    let replacement1 ←
+      tacenta_spqr.State.prepare_chains_capacity_loop self.chains replacement
+        0#usize
+    let _ ←
+      alloc.vec.Vec.Insts.ZeroizeZeroize.zeroize (Pair.Insts.ZeroizeZeroize
+        (zeroize.Zeroize.Blanket U64.Insts.ZeroizeDefaultIsZeroes)
+        tacenta_spqr.Chains.Insts.ZeroizeZeroize) self.chains
+    ok { self with chains := replacement1 }
+
 /-- [tacenta_session_unit::tacenta_spqr::{tacenta_session_unit::tacenta_spqr::State}::set_chains::closure]
-    Source: 'session-unit/src/../../spqr/src/lib.rs', lines 556:27-556:39 -/
+    Source: 'session-unit/src/../../spqr/src/lib.rs', lines 575:27-575:39 -/
 @[reducible]
 def tacenta_spqr.State.set_chains.closure := Std.U64
 
 /-- [tacenta_session_unit::tacenta_spqr::{tacenta_session_unit::tacenta_spqr::State}::set_chains::{impl core::ops::function::FnMut<(&'_ (u64, tacenta_session_unit::tacenta_spqr::Chains),), bool> for tacenta_session_unit::tacenta_spqr::{tacenta_session_unit::tacenta_spqr::State}::set_chains::closure<'_0>}::call_mut]:
-    Source: 'session-unit/src/../../spqr/src/lib.rs', lines 556:27-556:39 -/
+    Source: 'session-unit/src/../../spqr/src/lib.rs', lines 575:27-575:39 -/
 def
   tacenta_spqr.State.set_chains.closure.Insts.CoreOpsFunctionFnMutTupleSharedPairU64ChainsBool.call_mut
   (c : tacenta_spqr.State.set_chains.closure)
@@ -6698,7 +6747,7 @@ def
   ok (i != c, c)
 
 /-- [tacenta_session_unit::tacenta_spqr::{tacenta_session_unit::tacenta_spqr::State}::set_chains::{impl core::ops::function::FnOnce<(&'_ (u64, tacenta_session_unit::tacenta_spqr::Chains),), bool> for tacenta_session_unit::tacenta_spqr::{tacenta_session_unit::tacenta_spqr::State}::set_chains::closure<'_0>}::call_once]:
-    Source: 'session-unit/src/../../spqr/src/lib.rs', lines 556:27-556:39 -/
+    Source: 'session-unit/src/../../spqr/src/lib.rs', lines 575:27-575:39 -/
 def
   tacenta_spqr.State.set_chains.closure.Insts.CoreOpsFunctionFnOnceTupleSharedPairU64ChainsBool.call_once
   (c : tacenta_spqr.State.set_chains.closure)
@@ -6711,7 +6760,7 @@ def
   ok b
 
 /-- Trait implementation: [tacenta_session_unit::tacenta_spqr::{tacenta_session_unit::tacenta_spqr::State}::set_chains::{impl core::ops::function::FnOnce<(&'_ (u64, tacenta_session_unit::tacenta_spqr::Chains),), bool> for tacenta_session_unit::tacenta_spqr::{tacenta_session_unit::tacenta_spqr::State}::set_chains::closure<'_0>}]
-    Source: 'session-unit/src/../../spqr/src/lib.rs', lines 556:27-556:39 -/
+    Source: 'session-unit/src/../../spqr/src/lib.rs', lines 575:27-575:39 -/
 @[reducible]
 def
   tacenta_spqr.State.set_chains.closure.Insts.CoreOpsFunctionFnOnceTupleSharedPairU64ChainsBool
@@ -6722,7 +6771,7 @@ def
 }
 
 /-- Trait implementation: [tacenta_session_unit::tacenta_spqr::{tacenta_session_unit::tacenta_spqr::State}::set_chains::{impl core::ops::function::FnMut<(&'_ (u64, tacenta_session_unit::tacenta_spqr::Chains),), bool> for tacenta_session_unit::tacenta_spqr::{tacenta_session_unit::tacenta_spqr::State}::set_chains::closure<'_0>}]
-    Source: 'session-unit/src/../../spqr/src/lib.rs', lines 556:27-556:39 -/
+    Source: 'session-unit/src/../../spqr/src/lib.rs', lines 575:27-575:39 -/
 @[reducible]
 def
   tacenta_spqr.State.set_chains.closure.Insts.CoreOpsFunctionFnMutTupleSharedPairU64ChainsBool
@@ -6735,7 +6784,7 @@ def
 }
 
 /-- [tacenta_session_unit::tacenta_spqr::{tacenta_session_unit::tacenta_spqr::State}::set_chains]:
-    Source: 'session-unit/src/../../spqr/src/lib.rs', lines 555:4-558:5 -/
+    Source: 'session-unit/src/../../spqr/src/lib.rs', lines 574:4-578:5 -/
 def tacenta_spqr.State.set_chains
   (self : tacenta_spqr.State) (e : Std.U64) (c : tacenta_spqr.Chains) :
   Result tacenta_spqr.State
@@ -6744,16 +6793,19 @@ def tacenta_spqr.State.set_chains
     alloc.vec.Vec.retain Global
       tacenta_spqr.State.set_chains.closure.Insts.CoreOpsFunctionFnMutTupleSharedPairU64ChainsBool
       self.chains e
-  let v1 ← alloc.vec.Vec.push v (e, c)
-  ok { self with chains := v1 }
+  let self1 ←
+    tacenta_spqr.State.prepare_chains_capacity { self with chains := v }
+      1#usize
+  let v1 ← alloc.vec.Vec.push self1.chains (e, c)
+  ok { self1 with chains := v1 }
 
 /-- [tacenta_session_unit::tacenta_spqr::{tacenta_session_unit::tacenta_spqr::State}::clear_old_epochs::closure#1]
-    Source: 'session-unit/src/../../spqr/src/lib.rs', lines 566:20-566:69 -/
+    Source: 'session-unit/src/../../spqr/src/lib.rs', lines 586:20-586:69 -/
 @[reducible]
 def tacenta_spqr.State.clear_old_epochs.closure_1 := Std.U64
 
 /-- [tacenta_session_unit::tacenta_spqr::{tacenta_session_unit::tacenta_spqr::State}::clear_old_epochs::{impl core::ops::function::FnMut<(&'_ tacenta_session_unit::tacenta_spqr::Skipped,), bool> for tacenta_session_unit::tacenta_spqr::{tacenta_session_unit::tacenta_spqr::State}::clear_old_epochs::closure#1<'_0>}::call_mut]:
-    Source: 'session-unit/src/../../spqr/src/lib.rs', lines 566:20-566:69 -/
+    Source: 'session-unit/src/../../spqr/src/lib.rs', lines 586:20-586:69 -/
 def
   tacenta_spqr.State.clear_old_epochs.closure_1.Insts.CoreOpsFunctionFnMutTupleSharedSkippedBool.call_mut
   (c : tacenta_spqr.State.clear_old_epochs.closure_1)
@@ -6766,7 +6818,7 @@ def
   ok (c < i, c)
 
 /-- [tacenta_session_unit::tacenta_spqr::{tacenta_session_unit::tacenta_spqr::State}::clear_old_epochs::{impl core::ops::function::FnOnce<(&'_ tacenta_session_unit::tacenta_spqr::Skipped,), bool> for tacenta_session_unit::tacenta_spqr::{tacenta_session_unit::tacenta_spqr::State}::clear_old_epochs::closure#1<'_0>}::call_once]:
-    Source: 'session-unit/src/../../spqr/src/lib.rs', lines 566:20-566:69 -/
+    Source: 'session-unit/src/../../spqr/src/lib.rs', lines 586:20-586:69 -/
 def
   tacenta_spqr.State.clear_old_epochs.closure_1.Insts.CoreOpsFunctionFnOnceTupleSharedSkippedBool.call_once
   (c : tacenta_spqr.State.clear_old_epochs.closure_1)
@@ -6779,7 +6831,7 @@ def
   ok b
 
 /-- Trait implementation: [tacenta_session_unit::tacenta_spqr::{tacenta_session_unit::tacenta_spqr::State}::clear_old_epochs::{impl core::ops::function::FnOnce<(&'_ tacenta_session_unit::tacenta_spqr::Skipped,), bool> for tacenta_session_unit::tacenta_spqr::{tacenta_session_unit::tacenta_spqr::State}::clear_old_epochs::closure#1<'_0>}]
-    Source: 'session-unit/src/../../spqr/src/lib.rs', lines 566:20-566:69 -/
+    Source: 'session-unit/src/../../spqr/src/lib.rs', lines 586:20-586:69 -/
 @[reducible]
 def
   tacenta_spqr.State.clear_old_epochs.closure_1.Insts.CoreOpsFunctionFnOnceTupleSharedSkippedBool
@@ -6790,7 +6842,7 @@ def
 }
 
 /-- Trait implementation: [tacenta_session_unit::tacenta_spqr::{tacenta_session_unit::tacenta_spqr::State}::clear_old_epochs::{impl core::ops::function::FnMut<(&'_ tacenta_session_unit::tacenta_spqr::Skipped,), bool> for tacenta_session_unit::tacenta_spqr::{tacenta_session_unit::tacenta_spqr::State}::clear_old_epochs::closure#1<'_0>}]
-    Source: 'session-unit/src/../../spqr/src/lib.rs', lines 566:20-566:69 -/
+    Source: 'session-unit/src/../../spqr/src/lib.rs', lines 586:20-586:69 -/
 @[reducible]
 def
   tacenta_spqr.State.clear_old_epochs.closure_1.Insts.CoreOpsFunctionFnMutTupleSharedSkippedBool
@@ -6803,12 +6855,12 @@ def
 }
 
 /-- [tacenta_session_unit::tacenta_spqr::{tacenta_session_unit::tacenta_spqr::State}::clear_old_epochs::closure]
-    Source: 'session-unit/src/../../spqr/src/lib.rs', lines 564:20-564:65 -/
+    Source: 'session-unit/src/../../spqr/src/lib.rs', lines 584:20-584:65 -/
 @[reducible]
 def tacenta_spqr.State.clear_old_epochs.closure := Std.U64
 
 /-- [tacenta_session_unit::tacenta_spqr::{tacenta_session_unit::tacenta_spqr::State}::clear_old_epochs::{impl core::ops::function::FnMut<(&'_ (u64, tacenta_session_unit::tacenta_spqr::Chains),), bool> for tacenta_session_unit::tacenta_spqr::{tacenta_session_unit::tacenta_spqr::State}::clear_old_epochs::closure<'_0>}::call_mut]:
-    Source: 'session-unit/src/../../spqr/src/lib.rs', lines 564:20-564:65 -/
+    Source: 'session-unit/src/../../spqr/src/lib.rs', lines 584:20-584:65 -/
 def
   tacenta_spqr.State.clear_old_epochs.closure.Insts.CoreOpsFunctionFnMutTupleSharedPairU64ChainsBool.call_mut
   (c : tacenta_spqr.State.clear_old_epochs.closure)
@@ -6820,7 +6872,7 @@ def
   ok (c < i1, c)
 
 /-- [tacenta_session_unit::tacenta_spqr::{tacenta_session_unit::tacenta_spqr::State}::clear_old_epochs::{impl core::ops::function::FnOnce<(&'_ (u64, tacenta_session_unit::tacenta_spqr::Chains),), bool> for tacenta_session_unit::tacenta_spqr::{tacenta_session_unit::tacenta_spqr::State}::clear_old_epochs::closure<'_0>}::call_once]:
-    Source: 'session-unit/src/../../spqr/src/lib.rs', lines 564:20-564:65 -/
+    Source: 'session-unit/src/../../spqr/src/lib.rs', lines 584:20-584:65 -/
 def
   tacenta_spqr.State.clear_old_epochs.closure.Insts.CoreOpsFunctionFnOnceTupleSharedPairU64ChainsBool.call_once
   (c : tacenta_spqr.State.clear_old_epochs.closure)
@@ -6833,7 +6885,7 @@ def
   ok b
 
 /-- Trait implementation: [tacenta_session_unit::tacenta_spqr::{tacenta_session_unit::tacenta_spqr::State}::clear_old_epochs::{impl core::ops::function::FnOnce<(&'_ (u64, tacenta_session_unit::tacenta_spqr::Chains),), bool> for tacenta_session_unit::tacenta_spqr::{tacenta_session_unit::tacenta_spqr::State}::clear_old_epochs::closure<'_0>}]
-    Source: 'session-unit/src/../../spqr/src/lib.rs', lines 564:20-564:65 -/
+    Source: 'session-unit/src/../../spqr/src/lib.rs', lines 584:20-584:65 -/
 @[reducible]
 def
   tacenta_spqr.State.clear_old_epochs.closure.Insts.CoreOpsFunctionFnOnceTupleSharedPairU64ChainsBool
@@ -6844,7 +6896,7 @@ def
 }
 
 /-- Trait implementation: [tacenta_session_unit::tacenta_spqr::{tacenta_session_unit::tacenta_spqr::State}::clear_old_epochs::{impl core::ops::function::FnMut<(&'_ (u64, tacenta_session_unit::tacenta_spqr::Chains),), bool> for tacenta_session_unit::tacenta_spqr::{tacenta_session_unit::tacenta_spqr::State}::clear_old_epochs::closure<'_0>}]
-    Source: 'session-unit/src/../../spqr/src/lib.rs', lines 564:20-564:65 -/
+    Source: 'session-unit/src/../../spqr/src/lib.rs', lines 584:20-584:65 -/
 @[reducible]
 def
   tacenta_spqr.State.clear_old_epochs.closure.Insts.CoreOpsFunctionFnMutTupleSharedPairU64ChainsBool
@@ -6857,7 +6909,7 @@ def
 }
 
 /-- [tacenta_session_unit::tacenta_spqr::{tacenta_session_unit::tacenta_spqr::State}::clear_old_epochs]:
-    Source: 'session-unit/src/../../spqr/src/lib.rs', lines 562:4-567:5 -/
+    Source: 'session-unit/src/../../spqr/src/lib.rs', lines 582:4-587:5 -/
 def tacenta_spqr.State.clear_old_epochs
   (self : tacenta_spqr.State) (current : Std.U64) :
   Result tacenta_spqr.State
@@ -6873,7 +6925,7 @@ def tacenta_spqr.State.clear_old_epochs
   ok { self with chains := v, skipped := v1 }
 
 /-- [tacenta_session_unit::tacenta_spqr::{tacenta_session_unit::tacenta_spqr::State}::advance]:
-    Source: 'session-unit/src/../../spqr/src/lib.rs', lines 584:4-611:5 -/
+    Source: 'session-unit/src/../../spqr/src/lib.rs', lines 604:4-631:5 -/
 def tacenta_spqr.State.advance
   (self : tacenta_spqr.State) (out : tacenta_spqr.Output) :
   Result ((core.result.Result Unit tacenta_spqr.SpqrError) ×
@@ -6915,7 +6967,7 @@ def tacenta_spqr.State.advance
         ok (core.result.Result.Ok (), self2)
 
 /-- [tacenta_session_unit::tacenta_spqr::{tacenta_session_unit::tacenta_spqr::State}::maybe_advance]:
-    Source: 'session-unit/src/../../spqr/src/lib.rs', lines 613:4-618:5 -/
+    Source: 'session-unit/src/../../spqr/src/lib.rs', lines 633:4-638:5 -/
 def tacenta_spqr.State.maybe_advance
   (self : tacenta_spqr.State) (out : Option tacenta_spqr.Output) :
   Result ((core.result.Result Unit tacenta_spqr.SpqrError) ×
@@ -6926,7 +6978,7 @@ def tacenta_spqr.State.maybe_advance
   | some o => tacenta_spqr.State.advance self o
 
 /-- [tacenta_session_unit::tacenta_spqr::{tacenta_session_unit::tacenta_spqr::State}::send]:
-    Source: 'session-unit/src/../../spqr/src/lib.rs', lines 626:4-652:5
+    Source: 'session-unit/src/../../spqr/src/lib.rs', lines 646:4-672:5
     Visibility: public -/
 def tacenta_spqr.State.send
   (self : tacenta_spqr.State) (sending_epoch : Std.U64)
@@ -6970,7 +7022,7 @@ def tacenta_spqr.State.send
     ok (r1, self1)
 
 /-- [tacenta_session_unit::tacenta_spqr::{tacenta_session_unit::tacenta_spqr::State}::try_skipped]: loop body 0:
-    Source: 'session-unit/src/../../spqr/src/lib.rs', lines 658:8-665:5 -/
+    Source: 'session-unit/src/../../spqr/src/lib.rs', lines 678:8-685:5 -/
 @[rust_loop_body]
 def tacenta_spqr.State.try_skipped_loop.body
   (self : tacenta_spqr.State) (e : Std.U64) (n : Std.U64) (i : Std.Usize) :
@@ -7000,7 +7052,7 @@ def tacenta_spqr.State.try_skipped_loop.body
       self.direction))
 
 /-- [tacenta_session_unit::tacenta_spqr::{tacenta_session_unit::tacenta_spqr::State}::try_skipped]: loop 0:
-    Source: 'session-unit/src/../../spqr/src/lib.rs', lines 658:8-665:5 -/
+    Source: 'session-unit/src/../../spqr/src/lib.rs', lines 678:8-685:5 -/
 @[rust_loop]
 def tacenta_spqr.State.try_skipped_loop
   (self : tacenta_spqr.State) (e : Std.U64) (n : Std.U64) (i : Std.Usize) :
@@ -7013,7 +7065,7 @@ def tacenta_spqr.State.try_skipped_loop
     i
 
 /-- [tacenta_session_unit::tacenta_spqr::{tacenta_session_unit::tacenta_spqr::State}::try_skipped]:
-    Source: 'session-unit/src/../../spqr/src/lib.rs', lines 656:4-665:5 -/
+    Source: 'session-unit/src/../../spqr/src/lib.rs', lines 676:4-685:5 -/
 def tacenta_spqr.State.try_skipped
   (self : tacenta_spqr.State) (e : Std.U64) (n : Std.U64) :
   Result ((Option (Array Std.U8 32#usize)) × tacenta_spqr.State)
@@ -7023,45 +7075,9 @@ def tacenta_spqr.State.try_skipped
   ok (o, { rk := a, epoch := i, chains := v, skipped := v1, direction := d })
 
 /-- [tacenta_session_unit::tacenta_spqr::{tacenta_session_unit::tacenta_spqr::State}::skip_message_keys]: loop body 0:
-    Source: 'session-unit/src/../../spqr/src/lib.rs', lines 712:8-722:9 -/
+    Source: 'session-unit/src/../../spqr/src/lib.rs', lines 732:8-738:9 -/
 @[rust_loop_body]
 def tacenta_spqr.State.skip_message_keys_loop0.body
-  (e : Std.U64) (upto : Std.U64) (ck : Array Std.U8 32#usize)
-  (derived : alloc.vec.Vec tacenta_spqr.Skipped) (num : Std.U64) :
-  Result (ControlFlow ((Array Std.U8 32#usize) × (alloc.vec.Vec
-    tacenta_spqr.Skipped) × Std.U64) ((Array Std.U8 32#usize) ×
-    (alloc.vec.Vec tacenta_spqr.Skipped)))
-  := do
-  if num < upto
-  then
-    let num1 ← num + 1#u64
-    let (next, mk) ← tacenta_spqr.kdf_ck ck num1
-    let _ ←
-      Array.Insts.ZeroizeZeroize.zeroize (zeroize.Zeroize.Blanket
-        U8.Insts.ZeroizeDefaultIsZeroes) ck
-    let derived1 ←
-      alloc.vec.Vec.push derived ({ epoch := e, n := num1, key := mk } :
-        tacenta_spqr.Skipped)
-    ok (cont (next, derived1, num1))
-  else ok (done (ck, derived))
-
-/-- [tacenta_session_unit::tacenta_spqr::{tacenta_session_unit::tacenta_spqr::State}::skip_message_keys]: loop 0:
-    Source: 'session-unit/src/../../spqr/src/lib.rs', lines 712:8-722:9 -/
-@[rust_loop]
-def tacenta_spqr.State.skip_message_keys_loop0
-  (e : Std.U64) (upto : Std.U64) (ck : Array Std.U8 32#usize)
-  (derived : alloc.vec.Vec tacenta_spqr.Skipped) (num : Std.U64) :
-  Result ((Array Std.U8 32#usize) × (alloc.vec.Vec tacenta_spqr.Skipped))
-  := do
-  loop
-    (fun (ck1, derived1, num1) =>
-      tacenta_spqr.State.skip_message_keys_loop0.body e upto ck1 derived1 num1)
-    (ck, derived, num)
-
-/-- [tacenta_session_unit::tacenta_spqr::{tacenta_session_unit::tacenta_spqr::State}::skip_message_keys]: loop body 1:
-    Source: 'session-unit/src/../../spqr/src/lib.rs', lines 729:8-735:9 -/
-@[rust_loop_body]
-def tacenta_spqr.State.skip_message_keys_loop1.body
   (v : alloc.vec.Vec tacenta_spqr.Skipped) (e : Std.U64) (upto : Std.U64)
   (i : Std.U64) (skipped : alloc.vec.Vec tacenta_spqr.Skipped) (i1 : Std.Usize)
   :
@@ -7097,22 +7113,58 @@ def tacenta_spqr.State.skip_message_keys_loop1.body
     ok (cont (skipped1, i3))
   else ok (done skipped)
 
-/-- [tacenta_session_unit::tacenta_spqr::{tacenta_session_unit::tacenta_spqr::State}::skip_message_keys]: loop 1:
-    Source: 'session-unit/src/../../spqr/src/lib.rs', lines 729:8-735:9 -/
+/-- [tacenta_session_unit::tacenta_spqr::{tacenta_session_unit::tacenta_spqr::State}::skip_message_keys]: loop 0:
+    Source: 'session-unit/src/../../spqr/src/lib.rs', lines 732:8-738:9 -/
 @[rust_loop]
-def tacenta_spqr.State.skip_message_keys_loop1
+def tacenta_spqr.State.skip_message_keys_loop0
   (v : alloc.vec.Vec tacenta_spqr.Skipped) (e : Std.U64) (upto : Std.U64)
   (i : Std.U64) (skipped : alloc.vec.Vec tacenta_spqr.Skipped) (i1 : Std.Usize)
   :
   Result (alloc.vec.Vec tacenta_spqr.Skipped)
   := do
   loop
-    (fun (skipped1, i2) => tacenta_spqr.State.skip_message_keys_loop1.body v e
+    (fun (skipped1, i2) => tacenta_spqr.State.skip_message_keys_loop0.body v e
       upto i skipped1 i2)
     (skipped, i1)
 
+/-- [tacenta_session_unit::tacenta_spqr::{tacenta_session_unit::tacenta_spqr::State}::skip_message_keys]: loop body 1:
+    Source: 'session-unit/src/../../spqr/src/lib.rs', lines 744:8-754:9 -/
+@[rust_loop_body]
+def tacenta_spqr.State.skip_message_keys_loop1.body
+  (e : Std.U64) (upto : Std.U64) (skipped : alloc.vec.Vec tacenta_spqr.Skipped)
+  (ck : Array Std.U8 32#usize) (num : Std.U64) :
+  Result (ControlFlow ((alloc.vec.Vec tacenta_spqr.Skipped) × (Array Std.U8
+    32#usize) × Std.U64) ((alloc.vec.Vec tacenta_spqr.Skipped) × (Array
+    Std.U8 32#usize)))
+  := do
+  if num < upto
+  then
+    let num1 ← num + 1#u64
+    let (next, mk) ← tacenta_spqr.kdf_ck ck num1
+    let _ ←
+      Array.Insts.ZeroizeZeroize.zeroize (zeroize.Zeroize.Blanket
+        U8.Insts.ZeroizeDefaultIsZeroes) ck
+    let skipped1 ←
+      alloc.vec.Vec.push skipped ({ epoch := e, n := num1, key := mk } :
+        tacenta_spqr.Skipped)
+    ok (cont (skipped1, next, num1))
+  else ok (done (skipped, ck))
+
+/-- [tacenta_session_unit::tacenta_spqr::{tacenta_session_unit::tacenta_spqr::State}::skip_message_keys]: loop 1:
+    Source: 'session-unit/src/../../spqr/src/lib.rs', lines 744:8-754:9 -/
+@[rust_loop]
+def tacenta_spqr.State.skip_message_keys_loop1
+  (e : Std.U64) (upto : Std.U64) (skipped : alloc.vec.Vec tacenta_spqr.Skipped)
+  (ck : Array Std.U8 32#usize) (num : Std.U64) :
+  Result ((alloc.vec.Vec tacenta_spqr.Skipped) × (Array Std.U8 32#usize))
+  := do
+  loop
+    (fun (skipped1, ck1, num1) =>
+      tacenta_spqr.State.skip_message_keys_loop1.body e upto skipped1 ck1 num1)
+    (skipped, ck, num)
+
 /-- [tacenta_session_unit::tacenta_spqr::{tacenta_session_unit::tacenta_spqr::State}::skip_message_keys]:
-    Source: 'session-unit/src/../../spqr/src/lib.rs', lines 687:4-746:5 -/
+    Source: 'session-unit/src/../../spqr/src/lib.rs', lines 707:4-764:5 -/
 def tacenta_spqr.State.skip_message_keys
   (self : tacenta_spqr.State) (e : Std.U64) (upto : Std.U64) :
   Result ((core.result.Result Unit tacenta_spqr.SpqrError) ×
@@ -7145,19 +7197,16 @@ def tacenta_spqr.State.skip_message_keys
             ok (core.result.Result.Err tacenta_spqr.SpqrError.SkippedStoreFull,
               self)
           else
-            let i3 ← lift (UScalar.cast .Usize count)
-            let derived := alloc.vec.Vec.with_capacity tacenta_spqr.Skipped i3
-            let (ck, derived1) ←
-              tacenta_spqr.State.skip_message_keys_loop0 e upto ch1.ck derived
-                ch1.n
-            let i4 := alloc.vec.Vec.len self.skipped
-            let i5 ← lift (UScalar.cast .Usize count)
-            let i6 ← i4 + i5
-            let skipped := alloc.vec.Vec.with_capacity tacenta_spqr.Skipped i6
+            let i3 := alloc.vec.Vec.len self.skipped
+            let i4 ← lift (UScalar.cast .Usize count)
+            let i5 ← i3 + i4
+            let skipped := alloc.vec.Vec.with_capacity tacenta_spqr.Skipped i5
             let skipped1 ←
-              tacenta_spqr.State.skip_message_keys_loop1 self.skipped e upto
+              tacenta_spqr.State.skip_message_keys_loop0 self.skipped e upto
                 ch1.n skipped 0#usize
-            let (skipped2, _) ← alloc.vec.Vec.append Global skipped1 derived1
+            let (skipped2, ck) ←
+              tacenta_spqr.State.skip_message_keys_loop1 e upto skipped1 
+                ch1.ck ch1.n
             let o1 ←
               core.option.Option.Insts.CoreCloneClone.clone
                 tacenta_spqr.Chain.Insts.CoreCloneClone cs1.send
@@ -7167,7 +7216,7 @@ def tacenta_spqr.State.skip_message_keys
             ok (core.result.Result.Ok (), self1)
 
 /-- [tacenta_session_unit::tacenta_spqr::{tacenta_session_unit::tacenta_spqr::State}::receive]:
-    Source: 'session-unit/src/../../spqr/src/lib.rs', lines 760:4-798:5
+    Source: 'session-unit/src/../../spqr/src/lib.rs', lines 778:4-816:5
     Visibility: public -/
 def tacenta_spqr.State.receive
   (self : tacenta_spqr.State) (receiving_epoch : Std.U64)
@@ -7234,11 +7283,11 @@ def tacenta_spqr.State.receive
     ok (r1, self1)
 
 /-- [tacenta_session_unit::tacenta_spqr::STATE_VERSION]
-    Source: 'session-unit/src/../../spqr/src/lib.rs', lines 805:0-805:31 -/
+    Source: 'session-unit/src/../../spqr/src/lib.rs', lines 823:0-823:31 -/
 @[global_simps, irreducible] def tacenta_spqr.STATE_VERSION : Std.U8 := 1#u8
 
 /-- [tacenta_session_unit::tacenta_spqr::SpqrDecodeError]
-    Source: 'session-unit/src/../../spqr/src/lib.rs', lines 816:0-820:1
+    Source: 'session-unit/src/../../spqr/src/lib.rs', lines 834:0-838:1
     Visibility: public -/
 @[discriminant isize]
 inductive tacenta_spqr.SpqrDecodeError where
@@ -7247,7 +7296,7 @@ inductive tacenta_spqr.SpqrDecodeError where
 | Malformed : tacenta_spqr.SpqrDecodeError
 
 /-- [tacenta_session_unit::tacenta_spqr::{impl core::clone::Clone for tacenta_session_unit::tacenta_spqr::SpqrDecodeError}::clone]:
-    Source: 'session-unit/src/../../spqr/src/lib.rs', lines 815:9-815:14
+    Source: 'session-unit/src/../../spqr/src/lib.rs', lines 833:9-833:14
     Visibility: public -/
 def tacenta_spqr.SpqrDecodeError.Insts.CoreCloneClone.clone
   (self : tacenta_spqr.SpqrDecodeError) :
@@ -7256,7 +7305,7 @@ def tacenta_spqr.SpqrDecodeError.Insts.CoreCloneClone.clone
   ok self
 
 /-- Trait implementation: [tacenta_session_unit::tacenta_spqr::{impl core::clone::Clone for tacenta_session_unit::tacenta_spqr::SpqrDecodeError}]
-    Source: 'session-unit/src/../../spqr/src/lib.rs', lines 815:9-815:14 -/
+    Source: 'session-unit/src/../../spqr/src/lib.rs', lines 833:9-833:14 -/
 @[reducible]
 def tacenta_spqr.SpqrDecodeError.Insts.CoreCloneClone : core.clone.Clone
   tacenta_spqr.SpqrDecodeError := {
@@ -7264,7 +7313,7 @@ def tacenta_spqr.SpqrDecodeError.Insts.CoreCloneClone : core.clone.Clone
 }
 
 /-- Trait implementation: [tacenta_session_unit::tacenta_spqr::{impl core::marker::Copy for tacenta_session_unit::tacenta_spqr::SpqrDecodeError}]
-    Source: 'session-unit/src/../../spqr/src/lib.rs', lines 815:16-815:20 -/
+    Source: 'session-unit/src/../../spqr/src/lib.rs', lines 833:16-833:20 -/
 @[reducible]
 def tacenta_spqr.SpqrDecodeError.Insts.CoreMarkerCopy : core.marker.Copy
   tacenta_spqr.SpqrDecodeError := {
@@ -7272,14 +7321,14 @@ def tacenta_spqr.SpqrDecodeError.Insts.CoreMarkerCopy : core.marker.Copy
 }
 
 /-- Trait implementation: [tacenta_session_unit::tacenta_spqr::{impl core::marker::StructuralPartialEq for tacenta_session_unit::tacenta_spqr::SpqrDecodeError}]
-    Source: 'session-unit/src/../../spqr/src/lib.rs', lines 815:22-815:31 -/
+    Source: 'session-unit/src/../../spqr/src/lib.rs', lines 833:22-833:31 -/
 @[reducible]
 def tacenta_spqr.SpqrDecodeError.Insts.CoreMarkerStructuralPartialEq :
   core.marker.StructuralPartialEq tacenta_spqr.SpqrDecodeError := {
 }
 
 /-- [tacenta_session_unit::tacenta_spqr::{impl core::cmp::PartialEq<tacenta_session_unit::tacenta_spqr::SpqrDecodeError> for tacenta_session_unit::tacenta_spqr::SpqrDecodeError}::eq]:
-    Source: 'session-unit/src/../../spqr/src/lib.rs', lines 815:22-815:31
+    Source: 'session-unit/src/../../spqr/src/lib.rs', lines 833:22-833:31
     Visibility: public -/
 def tacenta_spqr.SpqrDecodeError.Insts.CoreCmpPartialEqSpqrDecodeError.eq
   (self : tacenta_spqr.SpqrDecodeError) (other : tacenta_spqr.SpqrDecodeError)
@@ -7291,7 +7340,7 @@ def tacenta_spqr.SpqrDecodeError.Insts.CoreCmpPartialEqSpqrDecodeError.eq
   ok (self1 = other1)
 
 /-- Trait implementation: [tacenta_session_unit::tacenta_spqr::{impl core::cmp::PartialEq<tacenta_session_unit::tacenta_spqr::SpqrDecodeError> for tacenta_session_unit::tacenta_spqr::SpqrDecodeError}]
-    Source: 'session-unit/src/../../spqr/src/lib.rs', lines 815:22-815:31 -/
+    Source: 'session-unit/src/../../spqr/src/lib.rs', lines 833:22-833:31 -/
 @[reducible]
 impl_def tacenta_spqr.SpqrDecodeError.Insts.CoreCmpPartialEqSpqrDecodeError :
   core.cmp.PartialEq tacenta_spqr.SpqrDecodeError tacenta_spqr.SpqrDecodeError
@@ -7302,14 +7351,14 @@ impl_def tacenta_spqr.SpqrDecodeError.Insts.CoreCmpPartialEqSpqrDecodeError :
 }
 
 /-- [tacenta_session_unit::tacenta_spqr::{impl core::cmp::Eq for tacenta_session_unit::tacenta_spqr::SpqrDecodeError}::assert_fields_are_eq]:
-    Source: 'session-unit/src/../../spqr/src/lib.rs', lines 815:33-815:35
+    Source: 'session-unit/src/../../spqr/src/lib.rs', lines 833:33-833:35
     Visibility: public -/
 def tacenta_spqr.SpqrDecodeError.Insts.CoreCmpEq.assert_fields_are_eq
   (self : tacenta_spqr.SpqrDecodeError) : Result Unit := do
   ok ()
 
 /-- Trait implementation: [tacenta_session_unit::tacenta_spqr::{impl core::cmp::Eq for tacenta_session_unit::tacenta_spqr::SpqrDecodeError}]
-    Source: 'session-unit/src/../../spqr/src/lib.rs', lines 815:33-815:35 -/
+    Source: 'session-unit/src/../../spqr/src/lib.rs', lines 833:33-833:35 -/
 @[reducible]
 def tacenta_spqr.SpqrDecodeError.Insts.CoreCmpEq : core.cmp.Eq
   tacenta_spqr.SpqrDecodeError := {
@@ -7320,7 +7369,7 @@ def tacenta_spqr.SpqrDecodeError.Insts.CoreCmpEq : core.cmp.Eq
 }
 
 /-- [tacenta_session_unit::tacenta_spqr::{impl core::fmt::Debug for tacenta_session_unit::tacenta_spqr::SpqrDecodeError}::fmt]:
-    Source: 'session-unit/src/../../spqr/src/lib.rs', lines 815:37-815:42
+    Source: 'session-unit/src/../../spqr/src/lib.rs', lines 833:37-833:42
     Visibility: public -/
 def tacenta_spqr.SpqrDecodeError.Insts.CoreFmtDebug.fmt
   (self : tacenta_spqr.SpqrDecodeError) (f : core.fmt.Formatter) :
@@ -7335,7 +7384,7 @@ def tacenta_spqr.SpqrDecodeError.Insts.CoreFmtDebug.fmt
     core.fmt.Formatter.write_str f (toStr "Malformed")
 
 /-- Trait implementation: [tacenta_session_unit::tacenta_spqr::{impl core::fmt::Debug for tacenta_session_unit::tacenta_spqr::SpqrDecodeError}]
-    Source: 'session-unit/src/../../spqr/src/lib.rs', lines 815:37-815:42 -/
+    Source: 'session-unit/src/../../spqr/src/lib.rs', lines 833:37-833:42 -/
 @[reducible]
 def tacenta_spqr.SpqrDecodeError.Insts.CoreFmtDebug : core.fmt.Debug
   tacenta_spqr.SpqrDecodeError := {
@@ -7343,14 +7392,14 @@ def tacenta_spqr.SpqrDecodeError.Insts.CoreFmtDebug : core.fmt.Debug
 }
 
 /-- [tacenta_session_unit::tacenta_spqr::CHAIN_LEN]
-    Source: 'session-unit/src/../../spqr/src/lib.rs', lines 825:0-825:36 -/
+    Source: 'session-unit/src/../../spqr/src/lib.rs', lines 843:0-843:36 -/
 @[global_simps, irreducible]
 def tacenta_spqr.CHAIN_LEN : Result Std.Usize := do
   let i ← 1#usize + 32#usize
   i + 8#usize
 
 /-- [tacenta_session_unit::tacenta_spqr::CHAINS_LEN]
-    Source: 'session-unit/src/../../spqr/src/lib.rs', lines 826:0-826:44 -/
+    Source: 'session-unit/src/../../spqr/src/lib.rs', lines 844:0-844:44 -/
 @[global_simps, irreducible]
 def tacenta_spqr.CHAINS_LEN : Result Std.Usize := do
   let i ← tacenta_spqr.CHAIN_LEN
@@ -7358,14 +7407,14 @@ def tacenta_spqr.CHAINS_LEN : Result Std.Usize := do
   8#usize + i1
 
 /-- [tacenta_session_unit::tacenta_spqr::SKIPPED_LEN]
-    Source: 'session-unit/src/../../spqr/src/lib.rs', lines 827:0-827:38 -/
+    Source: 'session-unit/src/../../spqr/src/lib.rs', lines 845:0-845:38 -/
 @[global_simps, irreducible]
 def tacenta_spqr.SKIPPED_LEN : Result Std.Usize := do
   let i ← 8#usize + 8#usize
   i + 32#usize
 
 /-- [tacenta_session_unit::tacenta_spqr::FIXED_PREFIX]
-    Source: 'session-unit/src/../../spqr/src/lib.rs', lines 829:0-833:8 -/
+    Source: 'session-unit/src/../../spqr/src/lib.rs', lines 847:0-851:8 -/
 @[global_simps, irreducible]
 def tacenta_spqr.FIXED_PREFIX : Result Std.Usize := do
   let i ← 1#usize + 32#usize
@@ -7374,7 +7423,7 @@ def tacenta_spqr.FIXED_PREFIX : Result Std.Usize := do
   i2 + 4#usize
 
 /-- [tacenta_session_unit::tacenta_spqr::{tacenta_session_unit::tacenta_spqr::Direction}::to_byte]:
-    Source: 'session-unit/src/../../spqr/src/lib.rs', lines 836:4-841:5 -/
+    Source: 'session-unit/src/../../spqr/src/lib.rs', lines 854:4-859:5 -/
 def tacenta_spqr.Direction.to_byte
   (self : tacenta_spqr.Direction) : Result Std.U8 := do
   match self with
@@ -7382,7 +7431,7 @@ def tacenta_spqr.Direction.to_byte
   | tacenta_spqr.Direction.B2a => ok 1#u8
 
 /-- [tacenta_session_unit::tacenta_spqr::{tacenta_session_unit::tacenta_spqr::Direction}::from_byte]:
-    Source: 'session-unit/src/../../spqr/src/lib.rs', lines 843:4-849:5 -/
+    Source: 'session-unit/src/../../spqr/src/lib.rs', lines 861:4-867:5 -/
 def tacenta_spqr.Direction.from_byte
   (b : Std.U8) : Result (Option tacenta_spqr.Direction) := do
   match b with
@@ -7391,7 +7440,7 @@ def tacenta_spqr.Direction.from_byte
   | _ => ok none
 
 /-- [tacenta_session_unit::tacenta_spqr::push_optional_chain]:
-    Source: 'session-unit/src/../../spqr/src/lib.rs', lines 852:0-865:1 -/
+    Source: 'session-unit/src/../../spqr/src/lib.rs', lines 870:0-883:1 -/
 def tacenta_spqr.push_optional_chain
   (out : alloc.vec.Vec Std.U8) (chain : Option tacenta_spqr.Chain) :
   Result (alloc.vec.Vec Std.U8)
@@ -7414,7 +7463,7 @@ def tacenta_spqr.push_optional_chain
     alloc.vec.Vec.extend_from_slice core.clone.CloneU8 out2 s1
 
 /-- [tacenta_session_unit::tacenta_spqr::decode_chain]: loop body 0:
-    Source: 'session-unit/src/../../spqr/src/lib.rs', lines 887:12-892:13 -/
+    Source: 'session-unit/src/../../spqr/src/lib.rs', lines 905:12-910:13 -/
 @[rust_loop_body]
 def tacenta_spqr.decode_chain_loop.body
   (i : Std.Usize) (bytes : Slice Std.U8) (pos : Std.Usize) (clean : Bool)
@@ -7433,7 +7482,7 @@ def tacenta_spqr.decode_chain_loop.body
   else ok (done clean)
 
 /-- [tacenta_session_unit::tacenta_spqr::decode_chain]: loop 0:
-    Source: 'session-unit/src/../../spqr/src/lib.rs', lines 887:12-892:13 -/
+    Source: 'session-unit/src/../../spqr/src/lib.rs', lines 905:12-910:13 -/
 @[rust_loop]
 def tacenta_spqr.decode_chain_loop
   (i : Std.Usize) (bytes : Slice Std.U8) (pos : Std.Usize) (clean : Bool)
@@ -7446,7 +7495,7 @@ def tacenta_spqr.decode_chain_loop
     (clean, i1)
 
 /-- [tacenta_session_unit::tacenta_spqr::decode_chain]:
-    Source: 'session-unit/src/../../spqr/src/lib.rs', lines 870:0-907:1 -/
+    Source: 'session-unit/src/../../spqr/src/lib.rs', lines 888:0-925:1 -/
 def tacenta_spqr.decode_chain
   (bytes : Slice Std.U8) (pos : Std.Usize) :
   Result (Option (Option tacenta_spqr.Chain))
@@ -7490,7 +7539,7 @@ def tacenta_spqr.decode_chain
     | _ => ok none
 
 /-- [tacenta_session_unit::tacenta_spqr::decode_chains_entry]:
-    Source: 'session-unit/src/../../spqr/src/lib.rs', lines 911:0-926:1 -/
+    Source: 'session-unit/src/../../spqr/src/lib.rs', lines 929:0-944:1 -/
 def tacenta_spqr.decode_chains_entry
   (bytes : Slice Std.U8) (pos : Std.Usize) :
   Result (Option (Std.U64 × tacenta_spqr.Chains))
@@ -7521,7 +7570,7 @@ def tacenta_spqr.decode_chains_entry
         ok (some (i4, { send := v, receive := v1 }))
 
 /-- [tacenta_session_unit::tacenta_spqr::decode_skipped_entry]:
-    Source: 'session-unit/src/../../spqr/src/lib.rs', lines 929:0-944:1 -/
+    Source: 'session-unit/src/../../spqr/src/lib.rs', lines 947:0-962:1 -/
 def tacenta_spqr.decode_skipped_entry
   (bytes : Slice Std.U8) (pos : Std.Usize) :
   Result (Option tacenta_spqr.Skipped)
@@ -7561,7 +7610,7 @@ def tacenta_spqr.decode_skipped_entry
     ok (some { epoch := i6, n := i7, key := key1 })
 
 /-- [tacenta_session_unit::tacenta_spqr::{tacenta_session_unit::tacenta_spqr::State}::encoded_len]:
-    Source: 'session-unit/src/../../spqr/src/lib.rs', lines 992:4-996:5 -/
+    Source: 'session-unit/src/../../spqr/src/lib.rs', lines 1010:4-1014:5 -/
 def tacenta_spqr.State.encoded_len
   (self : tacenta_spqr.State) : Result Std.Usize := do
   let i := alloc.vec.Vec.len self.chains
@@ -7576,7 +7625,7 @@ def tacenta_spqr.State.encoded_len
   i5 + i8
 
 /-- [tacenta_session_unit::tacenta_spqr::{tacenta_session_unit::tacenta_spqr::State}::to_bytes]: loop body 0:
-    Source: 'session-unit/src/../../spqr/src/lib.rs', lines 960:8-966:9
+    Source: 'session-unit/src/../../spqr/src/lib.rs', lines 978:8-984:9
     Visibility: public -/
 @[rust_loop_body]
 def tacenta_spqr.State.to_bytes_loop0.body
@@ -7601,7 +7650,7 @@ def tacenta_spqr.State.to_bytes_loop0.body
   else ok (done out)
 
 /-- [tacenta_session_unit::tacenta_spqr::{tacenta_session_unit::tacenta_spqr::State}::to_bytes]: loop 0:
-    Source: 'session-unit/src/../../spqr/src/lib.rs', lines 960:8-966:9
+    Source: 'session-unit/src/../../spqr/src/lib.rs', lines 978:8-984:9
     Visibility: public -/
 @[rust_loop]
 def tacenta_spqr.State.to_bytes_loop0
@@ -7614,7 +7663,7 @@ def tacenta_spqr.State.to_bytes_loop0
     (out, i)
 
 /-- [tacenta_session_unit::tacenta_spqr::{tacenta_session_unit::tacenta_spqr::State}::to_bytes]: loop body 1:
-    Source: 'session-unit/src/../../spqr/src/lib.rs', lines 969:8-975:9
+    Source: 'session-unit/src/../../spqr/src/lib.rs', lines 987:8-993:9
     Visibility: public -/
 @[rust_loop_body]
 def tacenta_spqr.State.to_bytes_loop1.body
@@ -7642,7 +7691,7 @@ def tacenta_spqr.State.to_bytes_loop1.body
   else ok (done out)
 
 /-- [tacenta_session_unit::tacenta_spqr::{tacenta_session_unit::tacenta_spqr::State}::to_bytes]: loop 1:
-    Source: 'session-unit/src/../../spqr/src/lib.rs', lines 969:8-975:9
+    Source: 'session-unit/src/../../spqr/src/lib.rs', lines 987:8-993:9
     Visibility: public -/
 @[rust_loop]
 def tacenta_spqr.State.to_bytes_loop1
@@ -7655,7 +7704,7 @@ def tacenta_spqr.State.to_bytes_loop1
     (out, j)
 
 /-- [tacenta_session_unit::tacenta_spqr::{tacenta_session_unit::tacenta_spqr::State}::to_bytes]:
-    Source: 'session-unit/src/../../spqr/src/lib.rs', lines 951:4-984:5
+    Source: 'session-unit/src/../../spqr/src/lib.rs', lines 969:4-1002:5
     Visibility: public -/
 def tacenta_spqr.State.to_bytes
   (self : tacenta_spqr.State) :
@@ -7689,7 +7738,7 @@ def tacenta_spqr.State.to_bytes
     (zeroize.Zeroize.Blanket U8.Insts.ZeroizeDefaultIsZeroes)) out8
 
 /-- [tacenta_session_unit::tacenta_spqr::{tacenta_session_unit::tacenta_spqr::State}::from_bytes]: loop body 0:
-    Source: 'session-unit/src/../../spqr/src/lib.rs', lines 1042:8-1050:9
+    Source: 'session-unit/src/../../spqr/src/lib.rs', lines 1060:8-1068:9
     Visibility: public -/
 @[rust_loop_body]
 def tacenta_spqr.State.from_bytes_loop0.body
@@ -7715,7 +7764,7 @@ def tacenta_spqr.State.from_bytes_loop0.body
       ok (cont (iter1, pos1, chains1, chains_ok))
 
 /-- [tacenta_session_unit::tacenta_spqr::{tacenta_session_unit::tacenta_spqr::State}::from_bytes]: loop 0:
-    Source: 'session-unit/src/../../spqr/src/lib.rs', lines 1042:8-1050:9
+    Source: 'session-unit/src/../../spqr/src/lib.rs', lines 1060:8-1068:9
     Visibility: public -/
 @[rust_loop]
 def tacenta_spqr.State.from_bytes_loop0
@@ -7733,7 +7782,7 @@ def tacenta_spqr.State.from_bytes_loop0
     (iter, pos, chains, chains_ok)
 
 /-- [tacenta_session_unit::tacenta_spqr::{tacenta_session_unit::tacenta_spqr::State}::from_bytes]: loop body 1:
-    Source: 'session-unit/src/../../spqr/src/lib.rs', lines 1069:8-1077:9
+    Source: 'session-unit/src/../../spqr/src/lib.rs', lines 1087:8-1095:9
     Visibility: public -/
 @[rust_loop_body]
 def tacenta_spqr.State.from_bytes_loop1.body
@@ -7758,7 +7807,7 @@ def tacenta_spqr.State.from_bytes_loop1.body
       ok (cont (iter1, pos1, skipped1, skipped_ok))
 
 /-- [tacenta_session_unit::tacenta_spqr::{tacenta_session_unit::tacenta_spqr::State}::from_bytes]: loop 1:
-    Source: 'session-unit/src/../../spqr/src/lib.rs', lines 1069:8-1077:9
+    Source: 'session-unit/src/../../spqr/src/lib.rs', lines 1087:8-1095:9
     Visibility: public -/
 @[rust_loop]
 def tacenta_spqr.State.from_bytes_loop1
@@ -7774,7 +7823,7 @@ def tacenta_spqr.State.from_bytes_loop1
     (iter, pos, skipped, skipped_ok)
 
 /-- [tacenta_session_unit::tacenta_spqr::{tacenta_session_unit::tacenta_spqr::State}::from_bytes]:
-    Source: 'session-unit/src/../../spqr/src/lib.rs', lines 1000:4-1103:5
+    Source: 'session-unit/src/../../spqr/src/lib.rs', lines 1018:4-1121:5
     Visibility: public -/
 def tacenta_spqr.State.from_bytes
   (bytes : Slice Std.U8) :
